TODO DNS updates.

examples/DnsServer/Dns.v
@@ -1,159 +1,318 @@
 Require Import AutoDB BagADT.
-Require Import Vector Ascii Bool Bvector List.
+Require Import Coq.Vectors.Vector Ascii Bool Bvector List.
 
-Definition name := list string.
+Section packet.
+  (* TODO: Move this section into a seperate file for basic
+     packet and DNS Record definitions. *)
 
-Inductive type := A | CNAME | NS | MX.
-Inductive class := IN | CH | HS.
+  Definition name := list string.
 
-Record question :=
-  { qname : name;
-    qtype : type;
-    qclass : class }.
+  Definition beq_name (a b : name) : bool :=
+    if (list_eq_dec string_dec a b) then true else false.
 
-Record answer :=
-  { aname : name;
-    atype : type;
-    aclass : class;
-    ttl : nat;
-    rdata : string }.
+  Lemma beq_name_dec
+  : forall (a b : name), beq_name a b = true <-> a = b.
+  Proof.
+    unfold beq_name; intros; find_if_inside; intuition; intros; congruence.
+  Qed.
 
-Record packet :=
-  { id : Bvector 16;
-    flags : Bvector 16;
-    questions : question; (* `list question` in case we can have multiple questions? *)
-    answers : list answer;
-    authority : list answer;
-    additional : list answer }.
+  Inductive RRecordType := A | CNAME | NS | MX.
 
-Definition sCOLLECTIONS := "Collections".
-Definition sNAME := "Name".
-Definition sTTL := "TTL".
-Definition sCLASS := "Class".
-Definition sTYPE := "Type".
-Definition sDATA := "Data".
+  Definition beq_RRecordType (a b : RRecordType) :=
+    match a, b with
+      | A, A => true
+      | CNAME, CNAME => true
+      | NS, NS => true
+      | MX, MX => true
+      | _, _ => false
+    end.
+  Lemma beq_RRecordType_dec
+  : forall (a b : RRecordType), beq_RRecordType a b = true <-> a = b.
+  Proof.
+    destruct a; destruct b; simpl; intuition; intros; congruence.
+  Qed.
+
+  (* Instances used in DecideableEnsemble. *)
+  Global Instance Query_eq_RRecordType :
+    Query_eq RRecordType.
+  Proof.
+    econstructor; decide equality.
+  Defined.
+
+  Inductive RRecordClass := IN | CH | HS.
+
+  Definition beq_RRecordClass (a b : RRecordClass) :=
+    match a, b with
+      | IN, IN => true
+      | CH, CH => true
+      | HS, HS => true
+      | _, _ => false
+    end.
+  Lemma beq_RRecordClass_dec
+  : forall (a b : RRecordClass), beq_RRecordClass a b = true <-> a = b.
+  Proof.
+    destruct a; destruct b; simpl; intuition; intros; congruence.
+  Qed.
+
+  (* Instances used in DecideableEnsemble. *)
+  Global Instance Query_eq_RRecordClass :
+    Query_eq RRecordClass.
+  Proof.
+    econstructor; decide equality.
+  Defined.
+
+  Record question :=
+    { qname : name;
+      qtype : RRecordType;
+      qclass : RRecordClass }.
+
+  Record answer :=
+    { aname : name;
+      atype : RRecordType;
+      aclass : RRecordClass;
+      ttl : nat;
+      rdata : string }.
+
+  Record packet :=
+    { id : Bvector 16;
+      flags : Bvector 16;
+      questions : question; (* `list question` in case we can have multiple questions? *)
+      answers : list answer;
+      authority : list answer;
+      additional : list answer }.
+
+  Lemma zero_lt_sixteen : lt 0 16. omega. Qed.
+  Definition buildempty (p : packet) :=
+    {| id := id p;
+       flags := replace_order (flags p) zero_lt_sixteen true; (* set QR bit *)
+       questions := questions p;
+       answers := [ ];
+       authority := [ ];
+       additional := [ ] |}.
+
+  Definition sCOLLECTIONS := "Collections".
+  Definition sNAME := "Name".
+  Definition sTTL := "TTL".
+  Definition sCLASS := "Class".
+  Definition sTYPE := "Type".
+  Definition sDATA := "Data".
+
+  (* DNS Resource Records. *)
+  Definition DNSRRecord :=
+    @Tuple <sNAME :: name,
+            sTYPE :: RRecordType,
+            sCLASS :: RRecordClass,
+            sTTL :: nat,
+            sDATA :: string>%Heading.
+
+  Definition toAnswer (t: DNSRRecord) :=
+    {| aname := t!sNAME;
+       atype := t!sTYPE;
+       aclass := t!sCLASS;
+       ttl := t!sTTL;
+       rdata := t!sDATA |}.
+
+  Definition addan (p : packet) (t : DNSRRecord) :=
+    {| id := id p;
+       flags := flags p;
+       questions := questions p;
+       answers := (toAnswer t) :: answers p;
+       authority := authority p;
+       additional := additional p |}.
+
+  Definition addns (p : packet) (t : DNSRRecord) :=
+    {| id := id p;
+       flags := flags p;
+       questions := questions p;
+       answers := answers p;
+       authority := (toAnswer t) :: (authority p);
+       additional := additional p |}.
+
+End packet.
 
 Definition DnsSchema :=
   Query Structure Schema
         [ relation sCOLLECTIONS has
                    schema <sNAME :: name,
-                           sTYPE :: type,
-                           sCLASS :: class,
-                           sTTL :: nat,
-                           sDATA :: string>
-          where (fun t t' =>
-                   t!sNAME = t'!sNAME -> t!sTYPE <> CNAME /\ t'!sTYPE <> CNAME)]
-        enforcing [ ].
+                      sTYPE :: RRecordType,
+                      sCLASS :: RRecordClass,
+                      sTTL :: nat,
+                      sDATA :: string>
+            where (fun t t' => t!sNAME = t'!sNAME -> t!sTYPE <> CNAME)]
+          enforcing [ ].
 
-Definition DnsTuple := TupleDef DnsSchema sCOLLECTIONS.
-Definition DnsSig : ADTSig :=
-  ADTsignature {
-      Constructor "Init" : unit -> rep,
-      Method "AddData" : rep x DnsTuple -> rep x bool,
-      Method "Process" : rep x packet -> rep x packet
+  Definition DnsSig : ADTSig :=
+    ADTsignature {
+        Constructor "Init" : unit -> rep,
+        Method "AddData" : rep x DNSRRecord -> rep x bool,
+        Method "Process" : rep x packet -> rep x packet
   }.
 
-Definition beq_string (p s : string) := if string_dec p s then true else false.
-
-Definition prefixProp (p s : name) := exists ps, List.app p ps = s.
+Definition prefixProp (p s : name) := exists ps, p ++ ps = s.
 Fixpoint prefixBool (p s : name) :=
   match p, s with
-    | List.nil, _ => true 
-    | List.cons p' ps', List.cons s' ss' => andb (beq_string p' s') (prefixBool ps' ss')
+    | [ ], _ => true
+    | p' :: ps', s' :: ss' => if string_dec p' s' then prefixBool ps' ss' else false
     | _, _ => false
   end.
 
-Definition upperbound (r : DnsTuple) (rs : list DnsTuple) :=
+Lemma prefixBool_eq :
+  forall (p s : name),
+    prefixBool p s = true -> prefixProp p s.
+Proof.
+  unfold prefixProp; induction p; intros s H.
+  - eexists s; reflexivity.
+  - destruct s; simpl in H.
+    + discriminate.
+    + find_if_inside; [subst | discriminate].
+      apply_in_hyp IHp; destruct_ex; eexists; subst; reflexivity.
+Qed.
+
+Definition upperbound (r : DNSRRecord) (rs : list DNSRRecord) :=
   forall r', List.In r' rs -> List.length r!sNAME >= List.length r'!sNAME.
 
-Lemma zero_lt_sixteen : lt 0 16. omega. Qed.
-Definition buildempty (p : packet) :=
-  {| id := id p;
-     flags := replace_order (flags p) zero_lt_sixteen true; (* set QR bit *)
-     questions := questions p;
-     answers := List.nil;
-     authority := List.nil;
-     additional := List.nil |}.
+Section FueledFix.
+  (* TODO: Find a home for these more definitions in the Common folder. *)
 
-Definition toAnswer (t: DnsTuple) :=
-  {| aname := t!sNAME;
-     atype := t!sTYPE;
-     aclass := t!sCLASS;
-     ttl := t!sTTL;
-     rdata := t!sDATA |}.
+  Variable A : Type. (* Argument Type *)
+  Variable R : Type. (* Return Type *)
 
-Definition addan (p : packet) (t : DnsTuple) :=
-  {| id := id p;
-     flags := flags p;
-     questions := questions p;
-     answers := (toAnswer t) :: answers p;
-     authority := authority p;
-     additional := additional p |}.
+  Fixpoint FueledFix (fuel : nat) (base : R) (body : (A -> R) -> A -> R) (arg : A)
+  : R :=
+    match fuel with
+      | O => base
+      | S fuel' => body (FueledFix fuel' base body) arg
+    end.
+End FueledFix.
 
-Definition addns (p : packet) (t : DnsTuple) :=
-  {| id := id p;
-     flags := flags p;
-     questions := questions p;
-     answers := answers p;
-     authority := (toAnswer t) :: (authority p);
-     additional := additional p |}.
+(* Can rewrite under Fueled Fix at the moment,
+as the condition on the body is not a proper relation. :p *)
+(* TODO: figure out a definition for pointwise_refine that is a
+   proper (i.e. reflexive and transitive) relation.
+ *)
 
-Fixpoint Fix A R (i : nat) (body : (A -> R) -> A -> R) (base : R) (arg : A) :=
-  match i with
-    | O => base
-    | S i' => body (Fix i' body base) arg
-  end.
+(* Definition pointwise_refine {A R}
+ (f g : (A -> Comp R) -> A -> Comp R) :=
+  forall (rec rec' : A -> Comp R) (a : A),
+    pointwise_relation A (@refine R) rec rec'
+    -> refine (f rec a) (g rec' a).
 
-Add Parametric Morphism A R i
-: (@Fix A (Comp R) i)
+Lemma reflexive_pR {A R : Type} :
+  forall A R, Reflexive (@pointwise_refine A R).
+Proof.
+  unfold Reflexive, pointwise_refine, pointwise_relation.
+  intros.
+  (* Doesn't work if x is (fun rec a => {r | ~ rec ~> r} :p *)
+Admitted.
+
+Lemma transitive_pR {A R : Type} :
+  forall A R, Transitive (@pointwise_refine A R).
+Proof.
+  unfold Transitive, pointwise_refine, pointwise_relation; intros.
+  etransitivity.
+  apply H; eauto.
+  apply H0. reflexivity.
+Qed. *)
+
+(* Add Parametric Morphism A R i
+: (@FueledFix A (Comp R) i)
     with signature
-    (fun f g => forall a a' r, (forall b, refine (a b) (a' b)) -> refine (f a r) (g a' r))
-      ==> (@refine R) 
+    ((@refine R)
+       ==> (@pointwise_refine A R)
       ==> (@eq A)
-      ==> (@refine R)
+      ==> (@refine R))
       as refineFix.
 Proof.
   simpl; induction i; intros; simpl.
   - assumption.
-  - apply H; apply IHi; [ apply H | apply H0 ].
-Qed.
+  - unfold pointwise_refine, pointwise_relation, Proper, respectful in *.
+    eapply H0.
+    intros.
+    generalize (IHi _ _ H _ _ H0 y1); clear.
+    apply H; apply IHi; [ apply H | apply H0 ].
+Qed. *)
 
-Arguments Fix : simpl never.
 
-Notation "'Filter' xs | p" := (Pick (fun xs' => forall x, List.In x xs' <-> List.In x xs /\ p x)) (at level 70) : comp_scope.
-Notation "'unique' b , p ->> s 'otherwise' ->> s'" := 
-  (Bind (Pick (fun b' => forall b, b' = Some b <-> p)) (fun b' =>
-   match b' with
-     | Some b => s
-     | None => s'
-   end)) (at level 70).
+(* TODO: Agree on a notation for our fueled fix function. *)
+Notation "'Repeat' fuel 'initializing' a 'with' arg 'defaulting' rec 'with' base {{ bod }} " :=
+  (FueledFix fuel base (fun rec a => bod) arg)
+    (no associativity, at level 50,
+     format "'Repeat' '[hv'  fuel  '/' 'initializing'  a  'with'  arg '/'  'defaulting'  rec  'with'  base  '/' {{ bod  }} ']' ").
+
+Section FueledFixRefinements.
+  (* TODO: Find a home for these refinements in the Computation folder. *)
+
+  Variable A : Type. (* Argument Type *)
+  Variable R : Type. (* Return Type *)
+
+  (* TODO Lemmas for refining FueledFix. *)
+
+  Lemma refine_FueledFix_Bind (B : Type) :
+    forall fuel body (base : Comp R) (arg : A) (k k' : R -> Comp B),
+      refine (r <- base; k r) (r <- base; k' r)
+      -> (forall fuel',
+            refine (a <- FueledFix fuel' base body arg; k a)
+                   (a <- FueledFix fuel' base body arg; k' a)
+            -> refine
+                 (a <- FueledFix (S fuel') base body arg; k a)
+                 (a <- FueledFix (S fuel') base body arg; k' a))
+      ->  refine (a <- FueledFix fuel base body arg; k a)
+                 (a <- FueledFix fuel base body arg; k' a).
+  Proof.
+    induction fuel; eauto.
+  Qed.
+
+End FueledFixRefinements.
+
+Section FilteredList.
+  (* TODO: Move FlattenComp to the Computation directory and find a
+     home for this definition. *)
+  Definition filtered_list {A}
+             (xs : list A)
+             (P : Ensemble A)
+    := FlattenCompList.flatten_CompList (map (fun x => Where (P x) (Return x)) xs).
+
+End FilteredList.
+
+Notation "[ x 'in' xs | P ]" := (filtered_list xs (fun x => P)) (at level 70) : comp_scope.
+
+(* Agree on this notation. *)
+Notation "'unique' b , P ->> s 'otherwise' ->> s'" :=
+  (b' <- {b' | forall b, b' = Some b <-> P};
+   (match b' with
+      | Some b => s
+      | None => s'
+    end)) (at level 70).
 
 Definition DnsSpec : ADT DnsSig :=
   QueryADTRep DnsSchema {
     Def Constructor "Init" (_ : unit) : rep := empty,
-    update "AddData" (t : DnsTuple) : bool :=
+    update "AddData" (t : DNSRRecord) : bool :=
       Insert t into sCOLLECTIONS,
     query "Process" (p : packet) : packet :=
       let t := qtype (questions p) in
-      Fix 7 (fun (rec : name -> Comp packet) (n : name)  =>
-         rs <- For (r in sCOLLECTIONS)
-            Where (prefixProp r!sNAME n)
-            Return r;
-         bfrs <- Filter rs | (fun x : DnsTuple => upperbound x rs);
-         b <- { b | decides b (forall r, List.In r bfrs -> n = r!sNAME) };
-         if b
-         then
-           unique b, List.In b bfrs /\ b!sTYPE = CNAME /\ t <> CNAME ->>
-             bfrs' <- Filter bfrs | (fun x : DnsTuple => x!sTYPE = t);
+      Repeat (*7 *) 1 initializing n with qname (questions p)
+                                                (* setting this to 1 until we work out the setoid *)
+                                                (* rewriting machinery *)
+               defaulting rec with (ret (buildempty p))
+         {{ rs <- For (r in sCOLLECTIONS)      (* Bind all the DNS entries whose names are *)
+                  Where (prefixProp r!sNAME n) (* a prefix of [n] to [rs] *)
+                  Return r;
+           bfrs <- [r in rs | upperbound r rs]; (* Find the best match (largest prefix) in [rs] *)
+           b <- { b | decides b (forall r, List.In r bfrs -> n = r!sNAME) };
+                            (* If there is an exact match *)
+           if b
+           then
+             unique b, List.In b bfrs /\ b!sTYPE = CNAME /\ t <> CNAME ->> (* *)
+             bfrs' <- [x in bfrs | x!sTYPE = t];
              p' <- rec b!sNAME;
              ret (List.fold_left addan bfrs' p')
            otherwise ->>
              ret (List.fold_left addan bfrs (buildempty p))
          else
-           bfrs' <- Filter bfrs | (fun x : DnsTuple => x!sTYPE = NS);
+           bfrs' <- [x in bfrs | x!sTYPE = NS];
            ret (List.fold_left addns bfrs' (buildempty p))
-      ) (ret (buildempty p)) (qname (questions p))
-  }.
+      }} }.
 
 Definition SearchTerm (s : name) (t : DnsSchema # sCOLLECTIONS) :=
   prefixBool (t!sNAME) s.
@@ -163,26 +322,395 @@ Definition DnsTerm :=
      BagUpdateTermType := name;
      BagApplyUpdateTerm := fun _ x => x |}.
 
+(* TODO : Move to appropriate files. *)
+    Global Instance DecideableEnsemble_NEqDec
+           {A B : Type}
+           {b_eq_dec : Query_eq B}
+           (f f' : A -> B)
+    : DecideableEnsemble (fun a : A => f a <> f' a) :=
+      {| dec a := if A_eq_dec (f a) (f' a) then false else true |}.
+    Proof.
+      intros; find_if_inside; intuition.
+    Qed.
+
+    Global Instance DecideableEnsemble_And
+           {A : Type}
+           {P P' : Ensemble A}
+           {P_dec : DecideableEnsemble P}
+           {P'_dec : DecideableEnsemble P'}
+    : DecideableEnsemble (fun a => P a /\ P' a) :=
+      {| dec a := DecideableEnsembles.dec (P := P) a
+                                          && DecideableEnsembles.dec (P := P') a |}.
+    Proof.
+      intros; rewrite <- (@DecideableEnsembles.dec_decides_P _ P),
+              <- (@DecideableEnsembles.dec_decides_P _ P').
+      setoid_rewrite andb_true_iff; reflexivity.
+    Qed.
+
+
+(* Parade of admitted refinement lemmas. Should go in a DNS Refinements file. *)
+
+    Lemma foo1 :
+      forall (n : DNSRRecord) (R : @IndexedEnsemble DNSRRecord),
+        n!sTYPE <> CNAME
+        -> refine {b |
+                   decides b
+                           (forall tup' : IndexedTuple,
+                              R tup' ->
+                              n!sNAME = (indexedElement tup')!sNAME -> n!sTYPE <> CNAME)}
+                  (ret true).
+    Proof.
+    Admitted.
+
+    Lemma foo2 :
+      forall (n : DNSRRecord) (R : @IndexedEnsemble DNSRRecord),
+        n!sTYPE = CNAME
+        -> refine {b |
+                   decides b
+                           (forall tup' : IndexedTuple,
+                              R tup' ->
+                              n!sNAME = (indexedElement tup')!sNAME -> n!sTYPE <> CNAME)}
+                  {b |
+                   decides b
+                           (exists tup' : IndexedTuple,
+                              R tup' /\
+                              n!sNAME = (indexedElement tup')!sNAME)}.
+    Proof.
+    Admitted.
+
+    Lemma foo4 :
+      forall (n : DNSRRecord) (R : @IndexedEnsemble DNSRRecord),
+        refine {b |
+                   decides b
+                           (forall tup' : IndexedTuple,
+                              R tup' ->
+                              (indexedElement tup')!sNAME = n!sNAME
+                              -> (indexedElement tup')!sTYPE <> CNAME)}
+                  {b |
+                   decides b
+                           (exists tup' : IndexedTuple,
+                              R tup' /\
+                              n!sNAME = (indexedElement tup')!sNAME
+                              /\ (indexedElement tup')!sTYPE <> CNAME)}.
+    Proof.
+    Admitted.
+
+    Lemma foo3 :
+      forall (n : DNSRRecord) (r : UnConstrQueryStructure DnsSchema),
+        refine {b |
+                decides b
+                        (forall tup' : @IndexedTuple (GetHeading DnsSchema sCOLLECTIONS),
+                           (r!sCOLLECTIONS)%QueryImpl tup' ->
+                           n!sNAME = (indexedElement tup')!sNAME -> n!sTYPE <> CNAME)}
+               (If (beq_RRecordType n!sTYPE CNAME)
+                   Then count <- Count
+                   For (UnConstrQuery_In r ``(sCOLLECTIONS)
+                                         (fun tup : Tuple =>
+                                            Where (n!sNAME = tup!sNAME)
+                                                  Return tup ));
+                ret (negb (beq_nat count 0)) Else ret true).
+    Proof.
+      intros; setoid_rewrite refine_pick_decides at 1;
+      [ | apply foo2 | apply foo1 ].
+      refine existence check into query.
+      remember n!sTYPE; refine pick val (beq_RRecordType d CNAME); subst;
+      [ | case_eq (beq_RRecordType n!sTYPE CNAME); intros;
+          rewrite <- beq_RRecordType_dec; unfold not; simpl in *; try congruence ].
+      simplify with monad laws.
+      reflexivity.
+    Qed.
+
+    Lemma foo5 :
+      forall (n : DNSRRecord) (r : UnConstrQueryStructure DnsSchema),
+        refine {b |
+                decides b
+                        (forall tup' : @IndexedTuple (GetHeading DnsSchema sCOLLECTIONS),
+                           (r!sCOLLECTIONS)%QueryImpl tup' ->
+                           (indexedElement tup')!sNAME = n!sNAME
+                           -> (indexedElement tup')!sTYPE <> CNAME)}
+               (count <- Count
+                   For (UnConstrQuery_In r ``(sCOLLECTIONS)
+                                         (fun tup : Tuple =>
+                                            Where (n!sNAME = tup!sNAME
+                                                   /\ tup!sTYPE <> CNAME )
+                                                  Return tup ));
+                ret (negb (beq_nat count 0))).
+    Proof.
+      intros; setoid_rewrite foo4.
+      refine existence check into query.
+      reflexivity.
+    Qed.
+
+    Lemma foo7 {heading}
+    : forall (R : Ensemble (@IndexedTuple heading))
+             (P : Ensemble Tuple)
+             (l : list Tuple),
+        For (QueryResultComp
+               R
+               (fun tup => Where (P tup)
+                                 (Return tup))) ↝ l  ->
+        forall (P' : Ensemble Tuple) (P'_dec : DecideableEnsemble P'),
+        refine (For (QueryResultComp
+                  R
+                  (fun tup => Where (P tup /\ P' tup)
+                                    (Return tup))))
+               (ret (filter DecideableEnsembles.dec l)).
+    Proof.
+      admit.
+    Qed.
+
+    Lemma foo8 {A}
+    : forall (c c' : bool) (t e e' : A),
+        (c = true -> c' = true)
+        -> (if c then (if c' then t else e) else e') = if c then t else e'.
+    Proof.
+      admit.
+    Qed.
+
+    Lemma foo9 {A}
+    : forall (l : list A) (pred : A -> bool),
+        negb (beq_nat (Datatypes.length l) 0) = true ->
+        negb (beq_nat (Datatypes.length (filter pred l)) 0) = true.
+    Proof.
+      admit.
+    Qed.
+
+    Transparent FueledFix.
+
 Theorem DnsManual :
   Sharpened DnsSpec.
 Proof.
   unfold DnsSpec.
   start honing QueryStructure.
 
+  (* Implement the constraint checks as queries. *)
+  hone method "AddData".
+  {
+    setoid_rewrite foo3.
+    setoid_rewrite foo5.
+    simplify with monad laws.
+    setoid_rewrite refine_If_Then_Else_Bind.
+    setoid_rewrite Bind_refine_If_Then_Else.
+    etransitivity.
+    apply refine_If_Then_Else_if.
+    - reflexivity.
+    - simplify with monad laws.
+      apply refine_under_bind; intros.
+      setoid_rewrite refine_Count; simplify with monad laws.
+      apply refine_under_bind; intros.
+      (* remove duplicate check *)
+      setoid_rewrite foo7; eauto.
+      simplify with monad laws.
+      rewrite foo8 by apply foo9.
+      higher_order_1_reflexivity.
+    - simplify with monad laws.
+      reflexivity.
+    - finish honing.
+  }
+
   hone representation using (@DelegateToBag_AbsR DnsSchema (icons DnsTerm (inil _))).
-  
+  (* TODO: We should define a 'make simple indexes' tactic notation variant for
+     prefix search terms. *)
+
   hone constructor "Init".
   {
     simplify with monad laws.
     rewrite refine_QSEmptySpec_Initialize_IndexedQueryStructure.
     finish honing.
   }
-  
+
   hone method "AddData".
+  {
+    etransitivity.
+    setoid_rewrite refine_If_Then_Else_Bind.
+    etransitivity.
+    - apply refine_If_Then_Else_if.
+      + reflexivity.
+      + simplify with monad laws.
+        setoid_rewrite refineEquiv_swap_bind.
+
+        implement_In.
+        convert_Where_to_search_term.
+        (* TODO: Find a search term to use here. *)
+        find_equivalent_search_term 0 find_simple_search_term.
+        convert_filter_to_find.
+        Implement_Aggregates.
+        simplify with monad laws.
+
+      implement_Insert_branches.
+
+        hone method "Process".
   {
     simplify with monad laws.
   }
-  
+
+
+      apply refine_bind; [ reflexivity
+                         | unfold pointwise_relation; intros].
+
+
+    setoid_rewrite refineEquiv_swap_bind.
+
+
+    Ltac Implement_If_Then_Else :=
+    match goal with
+      | |- refine (Bind (If ?i Then ?t Else ?e) ?k) _ =>
+        etransitivity;
+          [ apply (refine_If_Then_Else_Bind i t e k)
+          | etransitivity;
+            [ apply refine_If_Then_Else_if;
+              [ reflexivity | | ]
+            | ]
+          ]
+      | |- refine (If_Then_Else ?i (ret ?t) (ret ?e)) _ =>
+        etransitivity;
+          [ apply (refine_If_Then_Else_ret i t e)
+          | ]
+    end.
+
+    Implement_If_Then_Else.
+    simplify with monad laws.
+
+
+    idtac.
+
+      Focus 2.
+      setoid_rewrite r0.
+      simpl in *.
+
+
+      intuition eauto.
+      pattern (indexedElement x).
+      setoid_rewrite (r0 _ _ _).
+
+      pose (refine_constraint_check_into_query' (c:=r)
+                                                          (P':=fun tup' : @IndexedElement DNSRRecord =>
+                                                                 n!sNAME = (indexedElement tup')!sNAME)).
+
+      intros; apply foo1.
+      apply foo2.
+      eauto using foo1, foo2.
+      cut (sigT (refine {b0 : bool |
+                            decides b0
+                                    (exists tup' : IndexedTuple,
+                                       (r!sCOLLECTIONS)%QueryImpl tup' /\
+                                       n!sNAME = (indexedElement tup')!sNAME)})).
+      intros.
+      destruct X.
+      simpl in *.
+      etransitivity.
+      setoid_rewrite r0 at .
+      eapply refine_bind.
+
+      reflexivity.
+      setoid_rewrite r0.
+      simpl in *; unfold pointwise_relation; intros.
+      rewrite r0.
+      apply refine_If_Then_Else.
+      apply r0.
+
+      Add Parametric Morphism A (c : bool)
+      : (If_Then_Else c)
+          with signature
+          (@refine A ==> @refine A ==> @refine A )
+            as refine_If_Then_Else.
+      Proof.
+        unfold If_Then_Else; intros.
+        destruct c; eassumption.
+      Qed.
+
+      cut (refine (ret true) (ret false)).
+      intros.
+      cut (refine {b : bool |
+           decides b
+             (exists tup' : IndexedTuple,
+                (r!sCOLLECTIONS)%QueryImpl tup' /\
+                n!sNAME = (indexedElement tup')!sNAME)}
+          (ret true)); intros.
+      rewrite H0.
+      setoid_rewrite (refine_constraint_check_into_query' (c:=r)
+                                                          (P':=fun tup' : @IndexedElement DNSRRecord =>
+                                                                 n!sNAME = (indexedElement tup')!sNAME) _) at 1.
+
+      cut (Proper (refine ==> flip impl)
+                   (refine
+                      (If a
+                          Then {b : bool |
+                                decides b
+                                        (exists
+                                            tup' : IndexedTuple,
+                                                (r!sCOLLECTIONS)%QueryImpl
+                                                  tup' /\
+                                                n!sNAME =
+                                                (indexedElement tup')!sNAME)}
+                                      Else ret true))).
+      intros.
+      setoid_rewrite (refine_constraint_check_into_query' (c:=r)
+                                                          (P':=fun tup' : @IndexedElement DNSRRecord =>
+                                                                 n!sNAME = (indexedElement tup')!sNAME) _) at 1.
+
+      unfold Proper; simpl.
+      unfold respectful, flip, impl.
+      econstructor.
+      intros.
+
+
+      setoid_rewrite (refine_constraint_check_into_query' (c:=r)
+                                                          (P':=fun tup' : @IndexedElement DNSRRecord =>
+                                                                 n!sNAME = (indexedElement tup')!sNAME) _) at 1.
+
+      match goal with
+          |- context[{b | decides b
+                                  (exists tup : @IndexedTuple ?heading,
+                                     (GetUnConstrRelation ?qs ?tbl tup /\ @?P tup))}]
+          =>
+          pose (@refine_constraint_check_into_query' _ tbl qs P)
+      end.
+
+      setoid_rewrite (H _ _ _).
+      cut (DecideableEnsemble (fun tup' => n!sNAME = tup'!sNAME)).
+      cut (Same_set IndexedElement
+         (fun tup : IndexedElement =>
+          (fun tup' : Tuple => n!sNAME = tup'!sNAME) (indexedElement tup))
+         (fun tup' : IndexedTuple => n!sNAME = (indexedElement tup')!sNAME)).
+      intros.
+      pose (H _ X H0).
+      setoid_rewrite r0.
+      Check string_dec_bool_true_iff.
+        simpl; econstructor; intros;
+        try setoid_rewrite <- eq_nat_dec_bool_true_iff;
+        try setoid_rewrite <- eq_N_dec_bool_true_iff;
+        try setoid_rewrite <- eq_Z_dec_bool_true_iff;
+        try setoid_rewrite <- string_dec_bool_true_iff;
+        try setoid_rewrite and_True;
+        repeat progress (
+                 try setoid_rewrite <- andb_true_iff;
+                 try setoid_rewrite not_true_iff_false;
+                 try setoid_rewrite <- negb_true_iff).
+        rewrite bool_equiv_true;
+        reflexivity.
+      prove_decidability_for_functional_dependencies.
+      tauto_dec.
+      econstructor 1 with (fun b => if string_dec a b then true else false).
+      eauto with typeclass_instances.
+      setoid_rewrite (H (fun tup' => n!sNAME = tup'!sNAME)).
+      Focus 3.
+      reflexivity.
+
+    (Pick (fun (b : bool) =>
+                   decides b
+                           (exists tup2: @IndexedTuple _,
+                              (GetUnConstrRelation c tbl tup2 /\ P (indexedTuple tup2)))))
+
+        <-> ((n!sType = CNAME ->
+             exists (tup' : IndexedTuple),
+               (or!sCOLLECTIONS)%QueryImpl tup' /\
+               n!sNAME = (indexedElement tup')!sNAME)
+               /\ (n!sType <> CNAME -> True))
+
+    Implement_Insert_Checks.
+  }
+
   hone method "Process".
   {
     simplify with monad laws.
