src/QueryStructure/Specification/Representation/QueryStructureSchema.v
@@ -130,6 +130,11 @@ Instance Astring_eq : Query_eq string := {| A_eq_dec := string_dec |}.
 
 Instance Anat_eq : Query_eq nat := {| A_eq_dec := eq_nat_dec |}.
 
+Instance Query_eq_list {A : Type}
+         {a_eq_dec : Query_eq A}
+: Query_eq (list A) :=
+  {| A_eq_dec := list_eq_dec (@A_eq_dec A a_eq_dec) |}.
+
 Require Import Coq.NArith.NArith Coq.ZArith.ZArith.
 Instance AN_eq : Query_eq N := {| A_eq_dec := N.eq_dec |}.
 Instance AZ_eq : Query_eq Z := {| A_eq_dec := Z.eq_dec |}.
